CollapsingTowers/TwoLevelPCP/Store.lean
@@ -1,0 +1,4 @@
+
+import CollapsingTowers.TwoLevelPCP.Syntax
+abbrev Store :=
+  List Expr
